

## Lecture 9: Stability of Learning Algorithms

Lecturer: Abir De

Scribe: Group 2

## 9.1 Characterization of Stability of an Algorithm

Let  $A$  be a Learning Algorithm and  $S$  be the Data set which is fed into the Learning algorithm. The outcome/output of the learning algorithm is  $A(S)$ . (We can think of  $A(S)$  as a vector to define a norm)

**Definition 9.1.** (Stability) A learning algorithm  $A$  is said to be stable iff

$$\|A(S) - A(S')\| \leq \mathcal{O}\left(\frac{1}{|S|}\right)$$

For every  $S$  and  $S'$  such that  $|S \setminus S'| = |S' \setminus S| = 1$ .

The condition on  $S$  and  $S'$  means that there is only a one element mismatch between the sets.

Consider instead, what happens if we just delete one element  $e$  from the set and take the norm of the difference: (Stability towards single element deletions)

$$\|A(S) - A(S \setminus e)\|$$

We want to find the relation of the above with the previously defined notion of stability. This is dealt with in the following theorem.

**Proposition 9.2.** Let  $A$  be a Learning Algorithm,  $S = \{(x_i, y_i)\}$  be a data set and  $e$  be a single data point,  $e = (x_r, y_r)$  for some  $r$  such that  $e \in S$ . The following is a sufficient condition for the Algorithm to be stable:

$$\|A(S) - A(S \setminus e)\| = \mathcal{O}\left(\frac{1}{|S|}\right) \quad \forall e, S$$

*Proof.* Consider set  $S$  and  $S'$  such that  $|S \setminus S'| = |S' \setminus S| = 1$ . This means that there exists  $e$  and  $e'$  such that  $S \setminus e = S' \setminus e'$ . We shall also be using Triangle inequality. Let us start with the expression in the definition of stability:

$$\|A(S) - A(S')\| = \|A(S) - A(S \setminus e) + A(S' \setminus e') - A(S')\|$$

(We can do this since  $S \setminus e = S' \setminus e'$ ). Now applying Triangle inequality to the right hand side:

$$\|A(S) - A(S')\| \leq \|A(S) - A(S \setminus e)\| + \|A(S' \setminus e') - A(S')\|$$

But we already have :

$$\|A(S) - A(S \setminus e)\| = \mathcal{O}\left(\frac{1}{|S|}\right)$$

$$\|A(S' \setminus e') - A(S')\| = \mathcal{O}\left(\frac{1}{|S'|}\right)$$

Using this, we have:

$$\|A(S) - A(S')\| \leq \mathcal{O}\left(\frac{1}{|S|}\right) + \mathcal{O}\left(\frac{1}{|S'|}\right)$$

Since  $|S| = |S'|$  :

$$\|A(S) - A(S')\| \leq \mathcal{O}\left(\frac{1}{|S|}\right)$$

□

**Note:** If we add noise to  $x_i$  then accuracy will decrease, but our model will become more stable.

**Proposition 9.3.** *Let  $F_w(s) = \sum_{i \in S} [l(W^T x_i, y_i) + \lambda \|W\|^2]$  be the loss function of a Learning Algorithm,  $S = \{(x_i, y_i)\}$  be a data set where  $l$  is convex (i.e., all eigenvalues of  $\frac{\partial^2 l(W)}{\partial W^2}$  are positive) and Lipschitz continuous (i.e.,  $\|l(s) - l(s')\| \leq \|s - s'\|$ ). Then the Algorithm will be stable i.e.,*

$$\|W^*(S) - W^*(S')\| = \mathcal{O}\left(\frac{1}{|S|}\right)$$

where

$$W^* = \arg \min_W F_W(S)$$

*Proof.* If we are somehow able to prove below inequality

$$K \|W^*(S) - W^*(S')\|^2 \leq F_{w^*(s)}(S) - F_{w^*(s')}(S') \leq K' \|W^*(S) - W^*(S')\|$$

Then

$$K \|W^*(S) - W^*(S')\|^2 \leq K' \|W^*(S) - W^*(S')\|$$

$$\|W^*(S) - W^*(S')\| \leq K'/K$$

and now if we prove

$$K'/K = \mathcal{O}\left(\frac{1}{|S|}\right)$$

then as our requirement we are at the end of proof i.e.

$$\|W^*(S) - W^*(S')\| = \mathcal{O}\left(\frac{1}{|S|}\right)$$

To begin with that take a function  $g$  and assume  $g$  is convex.

So, from Taylor Series

$$g(W) = g(W_{min}) + (dg/dW_{min})^T (W - W_{min}) + (W - W_{min})^T \mathcal{H}(W - W_{min})$$

As

$$(dg/dW_{min}) = 0$$

and

$$\mathcal{H} \leq Eigen_{min}$$

we have

$$g(W) - g(W_{min}) \leq Eigen_{min}(W - W_{min})$$

Now take  $g$  is Lipschitz Continuous,

$$\|g(W) - g(W_{min})\| \leq L\|W - W_{min}\|$$

Here,

$$F_w(s) = \sum_{i \in S} [l(W^T x_i, y_i) + \lambda \|W\|^2]$$

So,

$$\mathcal{H} \geq 2\lambda S$$

and  $K$  is related to  $Eigen_{min} \geq \mathcal{H}$  i.e.  $K \approx 2\lambda S$

Now, we again start with

$$\begin{aligned} & F_{w^*(s)}(S) - F_{w^*(s')}(S') \\ &= F_{w^*(s)}(S) - F_{w^*(s)}(S') + F_{w^*(s)}(S') - F_{w^*(s')}(S') \\ &\leq F_{w^*(s')}(S) - F_{w^*(s')}(S') \\ &= l(W^*(S')^T x_i, y_i) - l(W^*(S)^T x'_i, y'_i) \\ &\leq L\|W^*(S') - W^*(S)\| \end{aligned}$$

by applying the triangular inequality and using the Lipschitz condition

□

## 9.2 Group Details and Individual Contribution

- 200110055 Keshav Patel Keval: Definition 9.1 and Proposition 9.2
- 19D070017 Bhavishya: Proposition 9.3
- 200100127 Rahul: Part of the Proof for Proposition 9.3
- 19D070046 Phansalkar Ishan Shrirang: Completed Proof for Proposition 9.3